pulse/ulib/experimental/Steel.Utils.fst
@@ -33,3 +33,43 @@ let pts_to_not_null (#a:Type)
     (fun _ -> True)
     (fun _ _ _ -> r =!= null)
   = lift_lemma (pts_to r p v) (r =!= null) (fun m -> Steel.Reference.pts_to_not_null r p v m)
+
+let change_slprop_ens (p:slprop) (q:slprop) (r:prop) (f:(m:mem -> Lemma (requires interp p m)
+                                                                       (ensures interp q m /\ r)))
+  : Steel unit p (fun _ -> q) (requires fun _ -> True) (ensures fun _ _ _ -> r)
+  = Steel.Effect.change_slprop p (q `star` pure r)
+                                 (fun m -> f m;
+                                        Steel.Memory.emp_unit q;
+                                        Steel.Memory.pure_star_interp q r m);
+    Steel.Utils.elim_pure r
+
+
+let pure_as_ens (#[@@framing_implicit] p:prop) ()
+  : Steel unit (pure p) (fun _ -> pure p) (fun _ -> True) (fun _ _ _ -> p)
+  = change_slprop_ens (pure p) (pure p) p (Steel.Memory.pure_interp p)
+
+let slassert (p:slprop)
+  : SteelT unit p (fun _ -> p)
+  = noop()
+
+let pts_to_injective_eq #a #p #q (r:ref a) (v0 v1:Ghost.erased a)
+  : Steel unit (pts_to r p v0 `star` pts_to r q v1)
+               (fun _ -> pts_to r p v0 `star` pts_to r q v0)
+               (requires fun _ -> True)
+               (ensures fun _ _ _ -> v0 == v1)
+  = change_slprop_ens (pts_to r p v0 `star` pts_to r q v1)
+                      (pts_to r p v0 `star` pts_to r q v0)
+                      (v0 == v1)
+                      (pts_to_ref_injective r p q v0 v1)
+
+module H = Steel.HigherReference
+let higher_ref_pts_to_injective_eq #a #p #q (r:H.ref a) (v0 v1:Ghost.erased a)
+  : Steel unit (H.pts_to r p v0 `star` H.pts_to r q v1)
+               (fun _ -> H.pts_to r p v0 `star` H.pts_to r q v0)
+               (requires fun _ -> True)
+               (ensures fun _ _ _ -> v0 == v1)
+  = let open H in
+    change_slprop_ens (pts_to r p v0 `star` pts_to r q v1)
+                      (pts_to r p v0 `star` pts_to r q v0)
+                      (v0 == v1)
+                      (pts_to_ref_injective r p q v0 v1)
